Completed LamConv bvar case

Auto/Embedding/LCtx.lean
@@ -5,21 +5,21 @@ namespace Auto.Embedding
 | 0     => x
 | n + 1 => lctx n
 
-def pushLCtx.comm (lctx : Nat → α) (f : α → β) (x : α) :
+def pushLCtx.comm (f : α → β) (lctx : Nat → α) (x : α) :
   (n : Nat) → f (pushLCtx lctx x n) = pushLCtx (fun n => f (lctx n)) (f x) n
 | 0       => rfl
 | .succ _ => rfl
 
-theorem pushLCtx.commFn  (lctx : Nat → α) (f : α → β) (x : α) :
+theorem pushLCtx.commFn (f : α → β) (lctx : Nat → α) (x : α) :
   (fun n => f (pushLCtx lctx x n)) = (fun n => pushLCtx (fun n => f (lctx n)) (f x) n) :=
-  funext (pushLCtx.comm lctx f x)
+  funext (pushLCtx.comm f lctx x)
 
-def pushLCtx.comm_cast₁ (lctx : Nat → α) (f : α → β) (g : β → Sort w) (x : α) :
+def pushLCtx.comm_cast₁ (f : α → β) (lctx : Nat → α) (g : β → Sort w) (x : α) :
   (n : Nat) → (H : g (f (pushLCtx lctx x n))) → g (pushLCtx (fun n => f (lctx n)) (f x) n)
 | 0       => fun H => H
 | .succ _ => fun H => H
 
-def pushLCtx.comm_cast₂ (lctx : Nat → α) (f : α → β) (g : β → Sort w) (x : α) :
+def pushLCtx.comm_cast₂ (f : α → β) (lctx : Nat → α) (g : β → Sort w) (x : α) :
   (n : Nat) → (H : g (pushLCtx (fun n => f (lctx n)) (f x) n)) → g (f (pushLCtx lctx x n))
 | 0       => fun H => H
 | .succ _ => fun H => H
@@ -29,15 +29,26 @@ def pushLCtx.comm_cast₂ (lctx : Nat → α) (f : α → β) (g : β → Sort w
 | 0     => x
 | n + 1 => lctx n
 
+def pushLCtxDep.comm {α : Sort w} {β : α → Sort x} {rty : Nat → α} {lctxty : α → Sort u}
+  (f : ∀ (x : α), lctxty x → β x) (lctx : ∀ n, lctxty (rty n))
+  {xty : α} (x : lctxty xty) : (n : Nat) →
+  f _ (pushLCtxDep lctx x n) = pushLCtxDep (lctxty:=β) (fun n => f _ (lctx n)) (f xty x) n
+| 0 => rfl
+| _ + 1  => rfl
+
+def pushLCtxDep.absorbAux {rty : Nat → α} {lctxty : α → Sort u}
+  (lctx : ∀ n, lctxty (rty n)) {xty : α} (x : lctxty xty) :
+  (n : Nat) → HEq
+    (@pushLCtxDep _ rty lctxty lctx _ x n)
+    (@pushLCtxDep _ (lctxty ∘ rty) id lctx _ x n)
+| 0 => HEq.refl _
+| _ + 1 => HEq.refl _
+
 theorem pushLCtxDep.absorb {rty : Nat → α} {lctxty : α → Sort u}
   (lctx : ∀ n, lctxty (rty n)) {xty : α} (x : lctxty xty) :
   PSigmaEq (fun (α : Nat → Sort u) => (∀ (n : Nat), α n))
     (@pushLCtxDep _ rty lctxty lctx _ x) (@pushLCtxDep _ (lctxty ∘ rty) id lctx _ x) :=
-  PSigmaEq.of_heq _ (HEq.funext _ _ (fun u =>
-    match u with
-    | 0       => HEq.refl _
-    | .succ _ => HEq.refl _
-  )) (pushLCtx.commFn _ _ _)
+  PSigmaEq.of_heq _ (HEq.funext _ _ (pushLCtxDep.absorbAux _ _)) (pushLCtx.commFn _ _ _)
 
 def pushLCtxAt (lctx : Nat → α) (x : α) : (pos : Nat) → Nat → α
 | 0 => pushLCtx lctx x
@@ -46,6 +57,19 @@ def pushLCtxAt (lctx : Nat → α) (x : α) : (pos : Nat) → Nat → α
   | 0 => lctx 0
   | n' + 1 => pushLCtxAt (fun n => lctx (Nat.succ n)) x pos' n'
 
+def pushLCtxAt.comm (f : α → β) (lctx : Nat → α) (x : α) :
+  (pos : Nat) → (n : Nat) → f (pushLCtxAt lctx x pos n) = pushLCtxAt (f ∘ lctx) (f x) pos n
+| 0 => fun n => by
+  dsimp [pushLCtxAt]; apply pushLCtx.comm
+| pos' + 1 => fun n =>
+  match n with
+  | 0 => rfl
+  | n' + 1 => pushLCtxAt.comm f (fun n => lctx (Nat.succ n)) x pos' n'
+
+theorem pushLCtxAt.commFn (lctx : Nat → α) (f : α → β) (x : α) (pos : Nat) :
+  (fun n => f (pushLCtxAt lctx x pos n)) = (fun n => pushLCtxAt (fun n => f (lctx n)) (f x) pos n) :=
+  funext (pushLCtxAt.comm f lctx x pos)
+
 def pushLCtxAtDep {rty : Nat → α} {lctxty : α → Sort u}
   (lctx : ∀ n, lctxty (rty n)) {xty : α} (x : lctxty xty) : (pos : Nat) → (n : Nat) → lctxty (pushLCtxAt rty xty pos n)
 | 0 => pushLCtxDep lctx x
@@ -53,6 +77,33 @@ def pushLCtxAtDep {rty : Nat → α} {lctxty : α → Sort u}
   match n with
   | 0 => lctx 0
   | n' + 1 => pushLCtxAtDep (fun n => lctx (Nat.succ n)) x pos' n'
+
+def pushLCtxAtDep.comm {α : Sort w} {β : α → Sort x} {rty : Nat → α} {lctxty : α → Sort u}
+  (f : ∀ (x : α), lctxty x → β x) (lctx : ∀ n, lctxty (rty n))
+  {xty : α} (x : lctxty xty) : (pos : Nat) → (n : Nat) →
+    f _ (pushLCtxAtDep lctx x pos n) = pushLCtxAtDep (lctxty:=β) (fun n => f _ (lctx n)) (f xty x) pos n
+| 0 => fun _ => pushLCtxDep.comm _ _ _ _
+| pos' + 1 => fun n =>
+  match n with
+  | 0 => rfl
+  | n' + 1 => pushLCtxAtDep.comm f (fun n => lctx (Nat.succ n)) x pos' n'
+
+def pushLCtxAtDep.absorbAux {rty : Nat → α} {lctxty : α → Sort u}
+  (lctx : ∀ n, lctxty (rty n)) {xty : α} (x : lctxty xty) :
+  (pos : Nat) → (n : Nat) → HEq
+    (@pushLCtxAtDep _ rty lctxty lctx _ x pos n)
+    (@pushLCtxAtDep _ (lctxty ∘ rty) id lctx _ x pos n)
+| 0 => fun _ => pushLCtxDep.absorbAux _ _ _
+| pos' + 1 => fun n =>
+  match n with
+  | 0 => HEq.refl _
+  | n' + 1 => pushLCtxAtDep.absorbAux (fun n => lctx (.succ n)) x pos' n'
+
+theorem pushLCtxAtDep.absorb {rty : Nat → α} {lctxty : α → Sort u}
+  (lctx : ∀ n, lctxty (rty n)) {xty : α} (x : lctxty xty) (pos : Nat) :
+  PSigmaEq (fun (α : Nat → Sort u) => (∀ (n : Nat), α n))
+    (@pushLCtxAtDep _ rty lctxty lctx _ x pos) (@pushLCtxAtDep _ (lctxty ∘ rty) id lctx _ x pos) :=
+  PSigmaEq.of_heq _ (HEq.funext _ _ (pushLCtxAtDep.absorbAux _ _ _)) (pushLCtxAt.commFn _ _ _ _)
 
 def popLCtx (lctx : Nat → α) := fun n => lctx (n + 1)
 
