Auto/Embedding/LamConv.lean
@@ -98,73 +98,6 @@ def LamWF.fromBVarLifts {lamVarTy lctx} (rterm : LamTerm) (lvl : Nat)
       LamWF lamVarTy ⟨f, rterm, argTy⟩
     popLCtx.succ_cast₁ _ castIH _ IH
 
--- **Note**: This is the `.bvar` case for the following `LamWF.subst`
--- The `LamWF` of the `ofBVar` we've just destructed is equivalent to
---   `argTy::(idx)→lctx ⊢ (.bvar n) : (argTy::(idx)→lctx)[n]`
--- The `wfArg` is equivalent to saying
---  `lctx[idx:] ⊢ arg : argTy`
--- Which can be turned into
---  `lctx ⊢ (bVarLifts arg idx) : (argTy::(idx)→lctx)[idx]`
--- What we want is
---   1. n < idx : `lctx ⊢ (.bvar n) : lctx[n]`
---   2. n = idx : `lctx ⊢ (bVarLifts arg idx) : argTy`
---   3. n = n' + 1 > idx : `lctx ⊢ (.bvar n') : lctx[n']`
--- It helps to think of `lctx ⊢ (.bvar n) : lctx[n]` as being bvar lifted
---   from `lctx ⊢ (.bvar 0) : lctx[0]`
--- The required type is
---   `lctx ⊢ substed : (argTy::(idx)→lctx)[n]`
--- The required definitional equalities are
---   1. n < idx          ::   lctx[n]  == (argTy::(idx)→lctx)[n]
---   2. n = idx          ::   argTy    == (argTy::(idx)→lctx)[n]
---   3. n = n' + 1 > idx ::   lctx[n'] == (argTy::(idx)→lctx)[n]
--- The term will be defined recursively. So we will have the following situation:
--- 1. n >= idx, requires
---    `lctx ⊢ substed : (argTy::(2)→lctx)[4]`     (idx, n, lctx) := (2, 4, pop 0)
---    given `LamWF.ofBVarLifts wfArg ::: lctx ⊢ (bVarLifts arg 2) : (argTy::(2)→lctx)[4]`
---  i.e.
---    `lctx ⊢ substed : (lctx[0]::lctx[1]::argTy::lctx[2:])[4]`  := (2, 4, pop 0)
---    given `_ ::: lctx ⊢ (bVarLifts arg 2) : (lctx[0]::lctx[1]::argTy::lctx[2:])[4]`
---  This can be bvar lifted from
---    `lctx[1:] ⊢ substed : (lctx[1]::argTy::lctx[2:])[3]`       := (1, 3, pop 1)
---    given `_ ::: lctx[1:] ⊢ (bVarLifts arg 1) : (lctx[1]::argTy::lctx[2:])[3]`
---  This can in turn be bvar lifted from
---    `lctx[2:] ⊢ substed : (argTy::lctx[2:])[2]`                := (0, `n` = 2, pop 2)
---    given `_ ::: lctx[2:] ⊢ arg : (argTy::lctx[2:])[2]`
---  At this point, we should do `cases` on `n`.
---    (1). If `n = 0`, we should use `substed := arg`
---    (2). if `n = n' + 1`, we should use `substed := (.bvar n')`
--- 2. n < idx, requires
---    `lctx ⊢ substed : (argTy::(4)→lctx)[2]`     (idx, n, lctx) := (4, 2, pop 0)
---  i.e                                                          := (4, 2, pop 0)
---    `lctx ⊢ substed : (lctx[0]::lctx[1]::lctx[2]::lctx[3]::argTy::lctx[4:])[2]`
---  This can be bvar lifted from                                 := (3, 1, pop 1)
---    `lctx[1:] ⊢ substed : (lctx[1]::lctx[2]::lctx[3]::argTy::lctx[4:])[1]`
---  This can in turn be bvar lifted from                         := (`idx'` = 2, 0, pop 2)
---    `lctx[2:] ⊢ substed : (lctx[2]::lctx[3]::argTy::lctx[4])[0]`
---  At this point, it's clear that `substed := (.bvar 0)`
--- **TODO**: Can this function be represented by `pushLCtxDep`?
---           Furthermore, can other functions be represented by `pushLCtxDep`?
-private def LamWF.subst_bvarAux
-  {ltv : LamTyVal} {lctx : Nat → LamSort} {argTy : LamSort}
-  (arg : LamTerm) (pops : Nat) : (idx : Nat) → (n : Nat) →
-  (wfArg : LamWF ltv ⟨popLCtxs lctx pops, arg.bvarLifts idx, argTy⟩) → 
-  (substed : LamTerm) × LamWF ltv ⟨(popLCtxs lctx pops), substed, pushLCtxAt (popLCtxs lctx pops) argTy idx n⟩
-  | 0 => fun n =>
-    match n with
-    | 0 => fun wfArg =>
-      ⟨arg, wfArg⟩
-    | n' + 1 => fun wfArg =>
-      ⟨.bvar n', .ofBVar _⟩
-  | idx' + 1 => fun n =>
-    match n with
-    | 0 => fun wfArg =>
-      ⟨.bvar 0, .ofBVar _⟩
-    | n' + 1 => fun wfArg =>
-      let wfArg' : LamWF ltv _ :=
-        LamWF.fromBVarLift (lctx:=popLCtxs lctx pops) _ wfArg
-      let IH := LamWF.subst_bvarAux arg (Nat.succ pops) idx' n' wfArg'
-      ⟨IH.fst.bvarLift, LamWF.ofBVarLift _ IH.snd⟩
-
 -- Suppose we have `(λ x. func[body]) arg`
 --   and `body` is a subterm of `func` under `idx` levels of binders in `func`.
 --   We want to compute what `body` will become when we beta-reduce the whole term
@@ -180,7 +113,10 @@ def LamWF.subst (ltv : LamTyVal) (idx : Nat)
   (substed : LamTerm) × LamWF ltv ⟨lctx, substed, bodyTy⟩
 | lctx, _,     .ofAtom n => ⟨.atom n, .ofAtom _⟩
 | lctx, _,     .ofBase (b:=b) H => ⟨.base b, .ofBase H⟩
-| lctx, wfArg, .ofBVar n => LamWF.subst_bvarAux arg 0 idx n wfArg
+| lctx, wfArg, .ofBVar n =>
+  let lctxty := fun rty => (substed : LamTerm) × LamWF ltv { lctx := lctx, rterm := substed, rty := rty}
+  let arg' := LamTerm.bvarLifts arg idx
+  pushLCtxAtDep (rty:=lctx) (lctxty:=lctxty) (lctx := fun n => ⟨.bvar n, .ofBVar n⟩) (xty:=argTy) (x := ⟨arg', wfArg⟩) idx n
 | lctx, wfArg, .ofLam (argTy:=argTy') bodyTy' (body:=body') H =>
   let wfArg' := LamWF.ofBVarLift (lctx:=pushLCtx lctx argTy') _ wfArg
   let IHArg := LamWF.subst ltv (Nat.succ idx) _ _ _ _ _ wfArg' H
@@ -203,12 +139,15 @@ def LamWF.subst_correct.{u} (lval : LamValuation.{u})
   = LamTerm.interp lval lctxTy lctxTerm wfSubst.snd)
 | lctxTy, lctxTerm, wfArg, .ofAtom n => rfl
 | lctxTy, lctxTerm, wfArg, .ofBase b => rfl
-| lctxTy, lctxTerm, wfArg, .ofBVar n => by simp [subst, LamTerm.interp]; sorry
-  -- This seems to be implying that
-  -- 1. We should state a commutativity theorem about `pushLCtxAtDep`
-  -- 1. `LamWF.subst_bvarAux` should be expressed by `pushLCtxAtDep`
-| lctxTy, lctxTerm, wfArg, .ofLam (argTy:=argTy') bodyTy' (body:=body') H =>
-  sorry
+| lctxTy, lctxTerm, wfArg, .ofBVar n =>
+  let β := LamSort.interp lval.ilVal.tyVal
+  let lctxty := fun (rty : LamSort) => (t : LamTerm) × LamWF lval.ilVal.toLamTyVal ⟨lctxTy, t, rty⟩
+  let f := fun (rty : LamSort) (r : lctxty rty) => LamTerm.interp lval lctxTy lctxTerm r.snd
+  let lctx := fun n => (⟨LamTerm.bvar n, .ofBVar n⟩ : @Sigma LamTerm
+    (fun substed => LamWF lval.ilVal.toLamTyVal ⟨lctxTy, substed, lctxTy n⟩))
+  Eq.symm (pushLCtxAtDep.comm (β:=β) (lctxty:=lctxty) f lctx ⟨_, wfArg⟩ _ _)
+| lctxTy, lctxTerm, wfArg, .ofLam (argTy:=argTy') bodyTy' (body:=body') H => by
+  simp [subst, LamTerm.interp]; sorry
 | lctxTy, lctxTerm, wfArg, .ofApp argTy' HFn HArg =>
   sorry
 
